\documentclass{article}
\usepackage[utf8]{inputenc}

\usepackage{amsmath}

\begin{document}
\section*{\LARGE To Normal Form}
\begin{flalign*}
&\text{{\LARGE $((\lambda a.(\lambda b.b\ b)\ (\lambda b.b\ b))\ b)\ ((\lambda c.(c\ b))\ (\lambda a.a)) \rightarrow_\beta$}} && \\
&\text{{\LARGE $((\lambda b.b\ b)\ (\lambda b.b\ b))\ ((\lambda c.(c\ b))\ (\lambda a.a)) \rightarrow_\beta$}} && \\
&\text{{\LARGE $((\lambda b.b\ b)\ (\lambda b.b\ b))\ ((\lambda a.a)\ b) \rightarrow_\beta$}} && \\
&\text{{\LARGE $((\lambda b.b\ b)\ (\lambda b.b\ b))\ b$}} && \\
\end{flalign*}

\section*{\LARGE SKK = I}
\begin{flalign*}
&\text{{\LARGE $S\ K\ K \equiv (\lambda x\ y\ z.x\ z\ (y\ z))\ (\lambda x\ y.x)\ (\lambda x\ y.x) \rightarrow_\beta$}} && \\
&\text{{\LARGE $(\lambda y\ z.(\lambda x\ y.x)\ z\ (y\ z))\ (\lambda x\ y.x) \rightarrow_\beta$}} && \\
&\text{{\LARGE $\lambda z.(\lambda x\ y.x)\ z\ ((\lambda x\ y.x)\ z) \rightarrow_\beta$}} && \\
&\text{{\LARGE $\lambda z.(\lambda x\ y.x)\ z\ (\lambda y.z) \rightarrow_\beta$}} && \\
&\text{{\LARGE $\lambda z.(\lambda y.z)\ (\lambda y.z) \rightarrow_\beta$}} && \\
&\text{{\LARGE $\lambda z.z \equiv I$}} &&
\end{flalign*}

\end{document}